broke out nominal version to separate file

Stlc/SM.v
@@ -5,182 +5,12 @@ Require Import Stlc.Stlc_inf.
 
 Notation "[ z ~> u ] e" := (subst_exp u z e) (at level 68).
 
-
-(* Some of our proofs are by induction on the *size* of
-   terms. We use the Omega tactic to easily dispatch reasoning
-   about natural numbers. *)
-Require Import Omega.
+Require Import Stlc.Nominal.
 
 
-(*************************************************************)
-(*   A nominal representation of terms                       *)
-(*************************************************************)
 
-(* A named representation of STLC terms.
-   No debruijn indices, and binders include the names of free variables. *)
-
-Inductive n_exp : Set :=
- | n_var (x:var)
- | n_abs (x:var) (t:n_exp)
- | n_app (t1:n_exp) (t2:n_exp).
-
-(* We can swap variables: this operation is
-   symmetric: x becomes y and y becomes x. *)
-Notation swap_var := (fun (x:var) (y:var) (z:var) =>
-  if (z == x) then y else if (z == y) then x else z).
-
-(* The main insight of nominal representations:
-   We can rename variables, without capture, using a simple
-   structural induction. Note how the [n_abs} case
-   we swap all variables, both bound and free.
-
-   For example:
-
-      (swap x y) (\z. (x y)) = \x. (y x))
-
-      (swap x y) (\x. x) = \y.y
-
-      (swap x y) (\y. x) = \x.y
-
-
-*)
-Fixpoint swap (x:var) (y:var) (t:n_exp) : n_exp :=
-  match t with
-  | n_var z     => n_var (swap_var x y z)
-  | n_abs z t1  => n_abs (swap_var x y z) (swap x y t1)
-  | n_app t1 t2 => n_app (swap x y t1) (swap x y t2)
-  end.
-
-(* The free variable function needs to remove the
-   bound variable in the [n_abs] case. *)
-Fixpoint fv_nom (n : n_exp) : atoms :=
-  match n with
-  | n_var x => {{x}}
-  | n_abs x n => AtomSetImpl.remove x (fv_nom n)
-  | n_app n1 n2 => fv_nom n1 `union` fv_nom n2
-  end.
-
-(* We can also define the "alpha-equivalence" relation
-   that declares when two nominal terms are equivalent
-   (up to swapping).
-
-   Note the two different rules for [n_abs]: either the
-   binders are the same and we can directly compare the
-   bodies, or the binders differ, but we can swap one
-   side to make it look like the other.
-
- *)
-Inductive aeq : n_exp -> n_exp -> Prop :=
- | aeq_var : forall x,
-     aeq (n_var x) (n_var x)
- | aeq_abs_same : forall x n1 n2,
-     aeq n1 n2 -> aeq (n_abs x n1) (n_abs x n2)
- | aeq_abs_diff : forall x y n1 n2,
-     x <> y ->
-     x `notin` fv_nom n2 ->
-     aeq n1 (swap y x n2) ->
-     aeq (n_abs x n1) (n_abs y n2)
- | aeq_app : forall n1 n2 n1' n2',
-     aeq n1 n1' -> aeq n2 n2' ->
-     aeq (n_app n1 n2) (n_app n1' n2').
-
-Hint Constructors aeq.
-
-
-(* -------------------------------------------------------- *)
-(* An abstract machine for named terms                      *)
-
-Fixpoint get {A :Type} (x:atom) (l : list (atom * A)) : option A :=
-  match l with
-  | nil => None
-  | (y,a)::tl => if (x == y) then Some a else get x tl
-  end.
-
-
-(* The advantage of named terms is a much more efficient operational
-   semantics. We don't need to recurse terms, opening and closing each
-   binder. Instead, as long as the binder is "sufficiently fresh" we can use
-   the name as is, and only rename (via swapping) when absolutely
-   necessary. *)
-
-(* We also don't even need to use substitution for our semantics.  Our
-   abstract maching will work with configurations (see below) which consist of
-   a head (i.e. delayed substitution) a term, and a stack. *)
-
-Definition heap := list (atom * n_exp).
-
-Inductive frame : Set := | n_app2 : n_exp -> frame.
-Notation  stack := (list frame).
-
-Definition conf := (heap * n_exp * stack)%type.
-
-
-(* The (small-step) semantics is a function from configurations to
-   configurations, until completion or error. *)
-
-Inductive Step a := Error   : Step a
-                 | Done     : Step a
-                 | TakeStep : a -> Step a.
-
-Definition isVal (e : n_exp) :=
-  match e with
-  | n_abs _ _ => true
-  | _         => false
-  end.
-
-Definition machine_step (c : conf) : Step conf :=
-  match c with
-    (h, e, s) =>
-    if isVal e then
-      match s with
-      | nil => Done _
-      | n_app2 a :: s' =>
-        match e with
-        | n_abs x e =>
-          (* if the bound name [x] is not fresh, we need to rename it *)
-          if AtomSetProperties.In_dec x (dom h)  then
-            let (y,_) := atom_fresh (dom h) in
-            TakeStep _ ((y,a)::h, swap x y e, s')
-          else
-            TakeStep _ ((x,a)::h, e, s')
-        | _ => Error _ (* non-function applied to argument *)
-        end
-      end
-    else match e with
-         | n_var x => match get x h with
-                     | Some e  => TakeStep _ (h, e, s)
-                     | None    => Error _ (* Unbound variable *)
-                     end
-         | n_app e1 e2 => TakeStep _ (h, e1, n_app2 e2 :: s)
-         | _ => Error _ (* unreachable (value in nonValueStep) *)
-         end
-  end.
-
-Definition initconf (e : n_exp) : conf := (nil,e,nil).
-
-
-(*
-
-Example: evaluation of  "(\y. (\x. x) y) 0"
-
-     machine                                       corresponding term
-
-      {}, (\y. (\x. x) y) 0 , nil                  (\y. (\x. x) y) 0
-  ==> {}, (\y. (\x. x) y), n_app2 0 :: nil         (\y. (\x. x) y) 0
-  ==> {y -> 0}, (\x.x) y, nil                      (\x. x) 0
-  ==> {y -> 0}, (\x.x), n_app2 y :: nil            (\x. x) 0
-  ==> {y -> 0}, y , nil                            0
-  ==> {y -> 0}, 0 , nil                            0
-  ==> Done
-
-(Note that the machine takes extra steps compared to the
-substitution semantics.)
-
-*)
 
 (* ------------------------------------------- *)
-
-
 
 (* Translation from machine configurations to LN terms.
    For flexibility in the proof, we decode the
@@ -217,6 +47,20 @@ Definition decode (c:conf) : exp  :=
   end.
 
 
+
+(* -----------------------------------------  *)
+
+(* Here's our first result about our decoding: that the two
+   free variable functions agree. *)
+
+Lemma fv_nom_fv_exp_eq : forall n,
+    fv_nom n [=] fv_exp (nom_to_exp n).
+Proof.
+  induction n; intros; simpl; autorewrite with lngen; fsetdec.
+Qed.
+
+Hint Rewrite fv_nom_fv_exp_eq : lngen.
+Hint Resolve fv_nom_fv_exp_eq : lngen.
 
 (* -----------------------------------------  *)
 
@@ -297,34 +141,36 @@ Qed.
    of e are bound in the remainder of the heap.
 *)
 
-Inductive scoped_heap : heap -> Prop :=
-  | scoped_nil  : scoped_heap nil
+Inductive scoped_heap (D : atoms) : heap -> Prop :=
+  | scoped_nil  : scoped_heap D nil
   | scoped_cons : forall x e h,
-      x `notin` dom h ->
-      fv_exp (nom_to_exp e) [<=] dom h ->
-      scoped_heap h ->
-      scoped_heap ((x,e)::h).
+      x `notin` dom h \u D ->
+      fv_exp (nom_to_exp e) [<=] dom h \u D ->
+      scoped_heap D h ->
+      scoped_heap D ((x,e)::h).
 
 
-Lemma scoped_get : forall h D x e,
-  scoped_heap h ->
+Lemma scoped_get : forall h D1 D2 x e,
+  scoped_heap D1 h ->
   get x h = Some e ->
-  dom h [<=] D ->
-  fv_exp (nom_to_exp e) [<=] D.
+  dom h \u D1 [<=] D2 ->
+  fv_exp (nom_to_exp e) [<=] D2.
 Proof.
   induction 1; intros; default_simp.
   fsetdec.
   eapply IHscoped_heap; auto; fsetdec.
 Qed.
 
-Lemma apply_heap_get :  forall h x e,
-    scoped_heap h ->
+Lemma apply_heap_get :  forall h D x e,
+    scoped_heap D h ->
     get x h = Some e ->
     apply_heap h (var_f x) = apply_heap h (nom_to_exp e).
 Proof.
-  induction 1; intros; default_simp;
+  induction 1; intros; default_simp.
   rewrite subst_exp_fresh_eq; auto.
-  rewrite scoped_get with (D:= dom h); eauto with lngen.
+  rewrite H0. auto.
+  rewrite subst_exp_fresh_eq; auto.
+  rewrite scoped_get with (D2:= dom h\u D );  eauto with lngen.
 Qed.
 
 (* ------------------------------------------ *)
@@ -359,18 +205,6 @@ Qed.
 
 (* ------------------------------------------ *)
 
-(* Here's our first result about our decoding: that the two
-   free variable functions agree. *)
-
-Lemma fv_nom_fv_exp_eq : forall n,
-    fv_nom n [=] fv_exp (nom_to_exp n).
-Proof.
-  induction n; intros; simpl; autorewrite with lngen; fsetdec.
-Qed.
-
-Hint Rewrite fv_nom_fv_exp_eq : lngen.
-Hint Resolve fv_nom_fv_exp_eq : lngen.
-
 (* Next, we show that nominal terms are aeq iff they decode
    to the same LN terms.
 
@@ -401,96 +235,6 @@ Proof.
   induction e; default_simp.
 Qed.
 
-(* Properties about nominal terms. *)
-
-(* Some are straightforward to prove *)
-
-Lemma swap_id : forall n x,
-    swap x x n = n.
-Proof.
-  induction n; default_simp.
-Qed.
-
-Lemma swap_symmetric : forall n x y,
-    swap x y n = swap y x n.
-Proof.
-  induction n; default_simp.
-Qed.
-
-Lemma swap_involutive : forall n x y,
-    swap x y (swap x y n) = n.
-Proof.
-  induction n; default_simp.
-Qed.
-
-(* We will need these below. *)
-
-Lemma fv_nom_swap : forall z y n,
-  z `notin` fv_nom n ->
-  y `notin` fv_nom (swap y z n).
-Proof.
-  induction n; default_simp.
-Qed.
-
-Lemma shuffle_swap : forall w y n z,
-    w <> z -> y <> z ->
-    (swap w y (swap y z n)) = (swap w z (swap w y n)).
-Proof.
-  induction n; default_simp.
-Qed.
-
-(* Other proofs about nominal terms involve swapping to make sure that
-   the variable names are "fresh enough". In this case, we need to
-   strengthen our induction hypothesis.
- *)
-
-Fixpoint size (n : n_exp) : nat :=
-  match n with
-  | n_var x => 1
-  | n_abs x e => 1 + size e
-  | n_app e1 e2 => 1 + size e1 + size e2
-  end.
-
-Lemma swap_size_constant : forall x y n,
-    size (swap x y n) = size n.
-Proof.
-  induction n; simpl; auto.
-Qed.
-
-Hint Rewrite swap_size_constant.
-
-(*
-Lemma nominal_induction_size L :
-     forall n, forall t, size t <= n ->
-     forall P : n_exp -> Prop,
-    (forall x, P (n_var x)) ->
-    (forall x t, (forall y, y `notin` L -> P (swap x y t)) -> P (n_abs x t)) ->
-    (forall t1 t2, P t1 -> P t2 -> P (n_app t1 t2)) ->
-    P t.
-Proof.
-  induction n.
-  intros t SZ; destruct t; simpl in *; inversion SZ.
-  intros t SZ P VAR ABS APP; destruct t; simpl in *.
-  - auto.
-  - apply ABS.
-    intros y Fr.
-    apply IHn; eauto; rewrite swap_size_constant; try omega.
-  - apply APP.
-    apply IHn; eauto; omega.
-    apply IHn; eauto; omega.
-Qed.
-
-Definition nominal_induction
-  : forall (L : atoms) (P : n_exp -> Prop),
-    (forall x : atom, P (n_var x)) ->
-    (forall (x : atom) (t : n_exp),
-        (forall y : atom, y `notin` L -> P (swap x y t)) -> P (n_abs x t)) ->
-    (forall t1 t2 : n_exp, P t1 -> P t2 -> P (n_app t1 t2)) ->
-    forall t : n_exp, P t :=
-  fun L P VAR APP ABS t =>
-  nominal_induction_size L (size t) t ltac:(auto) P VAR APP ABS.
-
-*)
 
 Lemma swap_spec_aux : forall m t w y,
     size t <= m ->
@@ -591,22 +335,22 @@ Qed.
 
 (* --------------------------------------------------------------- *)
 
-Inductive scoped_conf : conf -> Prop :=
-  scoped_conf_witness : forall h e s,
-    scoped_heap h ->
-    fv_exp (nom_to_exp e) [<=] dom h ->
-    fv_stack s [<=] dom h ->
-    scoped_conf (h,e,s).
+Inductive scoped_conf : atoms -> conf -> Prop :=
+  scoped_conf_witness : forall D h e s,
+    scoped_heap D h ->
+    fv_exp (nom_to_exp e) [<=] dom h \u D ->
+    fv_stack s [<=] dom h \u D  ->
+    scoped_conf D (h,e,s).
 
 
 (* Could be zero or one steps! *)
-Lemma simulate_step : forall h e s h' e' s' ,
-    machine_step (h,e,s) = TakeStep _ (h',e',s') ->
-    scoped_conf (h,e,s) ->
+Lemma simulate_step : forall D h e s h' e' s' ,
+    machine_step (dom h \u D) (h,e,s) = TakeStep _ (h',e',s') ->
+    scoped_conf D (h,e,s) ->
     decode (h,e,s) = decode (h',e',s') \/
     step (decode (h,e,s)) (decode (h',e',s')).
 Proof.
-  intros h e s h' e' s' STEP SCOPE.
+  intros D h e s h' e' s' STEP SCOPE.
   inversion SCOPE; subst; clear SCOPE.
   simpl in *.
   destruct (isVal e) eqn:?.
@@ -637,6 +381,7 @@ Proof.
           eapply apply_heap_lc.
           auto with lngen.
 
+          rewrite H4. fsetdec.
        -- rewrite subst_exp_spec.
           rewrite apply_heap_open; auto with lngen.
 
@@ -649,7 +394,7 @@ Proof.
     + destruct (get x h) eqn:?; inversion STEP; subst; clear STEP.
       left.
       f_equal.
-      apply apply_heap_get; auto.
+      apply apply_heap_get with (D:= D); auto.
     + inversion STEP; subst; clear STEP.
       left.
       simpl.
@@ -657,11 +402,11 @@ Proof.
       auto.
 Qed.
 
-Lemma simulate_done : forall h e s,
-    machine_step (h,e,s) = Done _ ->
-    scoped_heap h ->
-    fv_exp (nom_to_exp e) [<=] dom h ->
-    fv_stack s [<=] dom h ->
+Lemma simulate_done : forall D h e s,
+    machine_step (dom h \u D) (h,e,s) = Done _ ->
+    scoped_heap D h ->
+    fv_exp (nom_to_exp e) [<=] dom h \u D ->
+    fv_stack s [<=] dom h \u D ->
     is_value (nom_to_exp e).
 Proof.
   intros.
@@ -678,11 +423,11 @@ Proof.
 Qed.
 
 
-
-Lemma machine_is_scoped: forall h e s h' e' s',
-    machine_step (h,e,s) = TakeStep _ (h',e',s') ->
-    scoped_heap h  /\ fv_exp (nom_to_exp e)  [<=] dom h  /\ fv_stack s [<=] dom h ->
-    scoped_heap h' /\ fv_exp (nom_to_exp e') [<=] dom h' /\ fv_stack s' [<=] dom h'.
+(*
+Lemma machine_is_scoped: forall D h e s h' e' s',
+    machine_step D (h,e,s) = TakeStep _ (h',e',s') ->
+    scoped_heap D h  /\ fv_exp (nom_to_exp e)  [<=] dom h \u D /\ fv_stack s [<=] dom h ->
+    scoped_heap D h' /\ fv_exp (nom_to_exp e') [<=] dom h' \u D /\ fv_stack s' [<=] dom h'.
 Proof.
   intros.
   simpl in H.
@@ -727,7 +472,7 @@ Proof.
     split; try fsetdec.
     simpl. fsetdec.
 Qed.
-
+*)
 
 (* TODO: completeness *)
 (*
