Stlc/Nominal.v
@@ -1,0 +1,270 @@
+Require Import Metalib.Metatheory.
+Require Import Metalib.LibLNgen.
+
+(* Some of our proofs are by induction on the *size* of
+   terms. We use the Omega tactic to easily dispatch reasoning
+   about natural numbers. *)
+Require Export Omega.
+
+
+(*************************************************************)
+(*   A nominal representation of terms                       *)
+(*************************************************************)
+
+(* A named representation of STLC terms.
+
+   Binders include the names of free variables. *)
+
+Inductive n_exp : Set :=
+ | n_var (x:var)
+ | n_abs (x:var) (t:n_exp)
+ | n_app (t1:n_exp) (t2:n_exp).
+
+(* We can swap variables: this operation is
+   symmetric: x becomes y and y becomes x. *)
+Notation swap_var := (fun (x:var) (y:var) (z:var) =>
+  if (z == x) then y else if (z == y) then x else z).
+
+(* The main insight of nominal representations:
+
+   We can rename variables, without capture, using a simple
+   structural induction. Note how the [n_abs} case
+   we swap all variables, both bound and free.
+
+   For example:
+
+      (swap x y) (\z. (x y)) = \x. (y x))
+
+      (swap x y) (\x. x) = \y.y
+
+      (swap x y) (\y. x) = \x.y
+
+*)
+Fixpoint swap (x:var) (y:var) (t:n_exp) : n_exp :=
+  match t with
+  | n_var z     => n_var (swap_var x y z)
+  | n_abs z t1  => n_abs (swap_var x y z) (swap x y t1)
+  | n_app t1 t2 => n_app (swap x y t1) (swap x y t2)
+  end.
+
+(* The free variable function needs to remove the
+   bound variable in the [n_abs] case. *)
+Fixpoint fv_nom (n : n_exp) : atoms :=
+  match n with
+  | n_var x => {{x}}
+  | n_abs x n => AtomSetImpl.remove x (fv_nom n)
+  | n_app n1 n2 => fv_nom n1 `union` fv_nom n2
+  end.
+
+(* We can also define the "alpha-equivalence" relation
+   that declares when two nominal terms are equivalent
+   (up to swapping).
+
+   Note the two different rules for [n_abs]: either the
+   binders are the same and we can directly compare the
+   bodies, or the binders differ, but we can swap one
+   side to make it look like the other.
+
+ *)
+Inductive aeq : n_exp -> n_exp -> Prop :=
+ | aeq_var : forall x,
+     aeq (n_var x) (n_var x)
+ | aeq_abs_same : forall x n1 n2,
+     aeq n1 n2 -> aeq (n_abs x n1) (n_abs x n2)
+ | aeq_abs_diff : forall x y n1 n2,
+     x <> y ->
+     x `notin` fv_nom n2 ->
+     aeq n1 (swap y x n2) ->
+     aeq (n_abs x n1) (n_abs y n2)
+ | aeq_app : forall n1 n2 n1' n2',
+     aeq n1 n1' -> aeq n2 n2' ->
+     aeq (n_app n1 n2) (n_app n1' n2').
+
+Hint Constructors aeq.
+
+(* -------------------------------------------------------- *)
+
+(* Properties about nominal terms. *)
+
+(* Some are straightforward to prove *)
+
+Lemma swap_id : forall n x,
+    swap x x n = n.
+Proof.
+  induction n; default_simp.
+Qed.
+
+Lemma swap_symmetric : forall n x y,
+    swap x y n = swap y x n.
+Proof.
+  induction n; default_simp.
+Qed.
+
+Lemma swap_involutive : forall n x y,
+    swap x y (swap x y n) = n.
+Proof.
+  induction n; default_simp.
+Qed.
+
+(* We will need these later! *)
+
+Lemma fv_nom_swap : forall z y n,
+  z `notin` fv_nom n ->
+  y `notin` fv_nom (swap y z n).
+Proof.
+  induction n; default_simp.
+Qed.
+
+Lemma shuffle_swap : forall w y n z,
+    w <> z -> y <> z ->
+    (swap w y (swap y z n)) = (swap w z (swap w y n)).
+Proof.
+  induction n; default_simp.
+Qed.
+
+(* Other proofs about nominal terms involve swapping to make sure that
+   variable names are "fresh enough". In this case, we need to strengthen our
+   induction hypothesis.
+ *)
+
+Fixpoint size (n : n_exp) : nat :=
+  match n with
+  | n_var x => 1
+  | n_abs x e => 1 + size e
+  | n_app e1 e2 => 1 + size e1 + size e2
+  end.
+
+Lemma swap_size_constant : forall x y n,
+    size (swap x y n) = size n.
+Proof.
+  induction n; simpl; auto.
+Qed.
+
+Hint Rewrite swap_size_constant.
+
+
+Local Ltac gather_atoms ::=
+  let A := gather_atoms_with (fun x : atoms => x) in
+  let B := gather_atoms_with (fun x : atom => singleton x) in
+  let D := gather_atoms_with (fun x : n_exp => fv_nom x) in
+  constr:(A `union` B `union` D).
+
+Lemma nominal_induction_size L :
+     forall n, forall t, size t <= n ->
+     forall P : n_exp -> Prop,
+    (forall x, P (n_var x)) ->
+    (forall x t, (forall y, y `notin` L -> P (swap x y t)) -> P (n_abs x t)) ->
+    (forall t1 t2, P t1 -> P t2 -> P (n_app t1 t2)) ->
+    P t.
+Proof.
+  induction n.
+  intros t SZ; destruct t; simpl in *; inversion SZ.
+  intros t SZ P VAR ABS APP; destruct t; simpl in *.
+  - auto.
+  - apply ABS.
+    intros y Fr.
+    apply IHn; eauto; rewrite swap_size_constant; try omega.
+  - apply APP.
+    apply IHn; eauto; omega.
+    apply IHn; eauto; omega.
+Qed.
+
+Definition nominal_induction
+  : forall (L : atoms) (P : n_exp -> Prop),
+    (forall x : atom, P (n_var x)) ->
+    (forall (x : atom) (t : n_exp),
+        (forall y : atom, y `notin` L -> P (swap x y t)) -> P (n_abs x t)) ->
+    (forall t1 t2 : n_exp, P t1 -> P t2 -> P (n_app t1 t2)) ->
+    forall t : n_exp, P t :=
+  fun L P VAR APP ABS t =>
+  nominal_induction_size L (size t) t ltac:(auto) P VAR APP ABS.
+
+(* -------------------------------------------------------- *)
+(* An abstract machine for cbn evaluation of named terms    *)
+
+Fixpoint get {A :Type} (x:atom) (l : list (atom * A)) : option A :=
+  match l with
+  | nil => None
+  | (y,a)::tl => if (x == y) then Some a else get x tl
+  end.
+
+
+(* The advantage of named terms is an efficient operational semantics! We
+   don't need to recurse terms, opening and closing each binder. Instead, as
+   long as the binder is "sufficiently fresh" we can use the name as is, and
+   only rename (via swapping) when absolutely necessary. *)
+
+(* We also don't even need to use substitution for our semantics.  Our
+   abstract maching will work with configurations (see below) which consist of
+   a head (i.e. delayed substitution) a term, and a stack. *)
+
+Definition heap := list (atom * n_exp).
+
+Inductive frame : Set := | n_app2 : n_exp -> frame.
+Notation  stack := (list frame).
+
+Definition conf := (heap * n_exp * stack)%type.
+
+
+(* The (small-step) semantics is a function from configurations to
+   configurations, until completion or error. *)
+
+Inductive Step a := Error   : Step a
+                 | Done     : Step a
+                 | TakeStep : a -> Step a.
+
+Definition isVal (e : n_exp) :=
+  match e with
+  | n_abs _ _ => true
+  | _         => false
+  end.
+
+Definition machine_step (avoid : atoms) (c : conf) : Step conf :=
+  match c with
+    (h, e, s) =>
+    if isVal e then
+      match s with
+      | nil => Done _
+      | n_app2 a :: s' =>
+        match e with
+        | n_abs x e =>
+          (* if the bound name [x] is not fresh, we need to rename it *)
+          if AtomSetProperties.In_dec x avoid  then
+            let (y,_) := atom_fresh avoid in
+             TakeStep _ ((y,a)::h, swap x y e, s')
+          else
+            TakeStep _ ((x,a)::h, e, s')
+        | _ => Error _ (* non-function applied to argument *)
+        end
+      end
+    else match e with
+         | n_var x => match get x h with
+                     | Some e  => TakeStep _ (h, e, s)
+                     | None    => Error _ (* Unbound variable *)
+                     end
+         | n_app e1 e2 => TakeStep _ (h, e1, n_app2 e2 :: s)
+         | _ => Error _ (* unreachable (value in nonValueStep) *)
+         end
+  end.
+
+Definition initconf (e : n_exp) : conf := (nil,e,nil).
+
+
+(*
+
+Example: evaluation of  "(\y. (\x. x) y) 0"
+
+     machine                                       corresponding term
+
+      {}, (\y. (\x. x) y) 0 , nil                  (\y. (\x. x) y) 0
+  ==> {}, (\y. (\x. x) y), n_app2 0 :: nil         (\y. (\x. x) y) 0
+  ==> {y -> 0}, (\x.x) y, nil                      (\x. x) 0
+  ==> {y -> 0}, (\x.x), n_app2 y :: nil            (\x. x) 0
+  ==> {y -> 0}, y , nil                            0
+  ==> {y -> 0}, 0 , nil                            0
+  ==> Done
+
+(Note that the machine takes extra steps compared to the
+substitution semantics.)
+
+*)
